$ P = \big( (a(\tau) + b(\tau) \delta + r(\tau) \delta^2) \epsilon \big) G $

$ K = \sum_{i \in [m]} k_{a,i} G_{K, 0, i} + k_{b,i} G_{K, 1, i} + \sum_{i \in [2 m]} k_{r,i} G_{K, 2, i}. $

Proof $\pi = (P, K, a_0, b_0)$

$ P - (a + \delta b + \delta^2 r) \epsilon G = (\tau - \alpha) \epsilon K $

$\mathcal{R} = \left\{ (\tau, \delta, \epsilon ; H_\tau, H_\delta, H_\epsilon, \pi) : \begin{array}{} H_x = x H \text{ for } x = \tau, \delta, \epsilon \\ P - (a + \delta b + \delta^2 r) \epsilon G = (\tau - \alpha) \epsilon K \end{array} \right\}$
